fiat-rust/src/secp256k1_montgomery_scalar_32.rs
@@ -5754,7 +5754,7 @@ pub const fn fiat_secp256k1_montgomery_scalar_divstep(out1: &mut u32, mut out2: 
 ///
 /// ```text
 /// Postconditions:
-///   eval (from_montgomery out1) = ⌊(m - 1) / 2⌋^(if ⌊log2 m⌋ + 1 < 46 then ⌊(49 * (⌊log2 m⌋ + 1) + 80) / 17⌋ else ⌊(49 * (⌊log2 m⌋ + 1) + 57) / 17⌋)
+///   eval (from_montgomery out1) = ⌊(m + 1) / 2⌋^(if ⌊log2 m⌋ + 1 < 46 then ⌊(49 * (⌊log2 m⌋ + 1) + 80) / 17⌋ else ⌊(49 * (⌊log2 m⌋ + 1) + 57) / 17⌋) mod m
 ///   0 ≤ eval out1 < m
 /// ```
 ///
